\documentclass{article}
\usepackage{amsmath}
\begin{document}

\section*{Problema 2}

Solutie \\\\

\noindent Vom afla $w^*$ calculând derivata parțială față de $w$ cu 0.

\noindent \[
\frac{\partial}{\partial w} \left( \frac{1}{m} \sum_{i=1}^{m} L(w^T x_i, y_i) + \frac{\lambda}{2} \|w\|^2 \right) = 0 \quad (1)
\]

\noindent \[
\Rightarrow \frac{\partial}{\partial w} \left( \frac{1}{m} \sum_{i=1}^{m} L(w^T x_i, y_i) \right) + \lambda w = 0 \quad (2)
\]

\noindent \[
\Rightarrow -\frac{1}{m} \sum_{i=1}^{m} \frac{\partial L}{\partial w} (w^T x_i, y_i) + \lambda w = 0 \quad (3)
\]

\noindent \[
\Rightarrow \lambda w = \frac{1}{m} \sum_{i=1}^{m} \frac{\partial L}{\partial w} (w^T x_i, y_i) \quad (4)
\]

\noindent \[
w^* = \frac{1}{\lambda m} \sum_{i=1}^{m} \frac{\partial L}{\partial w} (w^T x_i, y_i) \quad (5)
\]

\noindent \[
\frac{\partial L}{\partial w} (w^T x_i, y_i) = \frac{\partial L}{\partial z} (w^T x_i) x_i \quad (6)
\]

\noindent \[
\Rightarrow w^* = \frac{1}{\lambda m} \sum_{i=1}^{m} \frac{\partial L}{\partial z} (w^T x_i) x_i
\]

Q.E.D.

\end{document}
